Port full tactic to Selectors

examples/steel/Selectors.Tests.fst
@@ -5,6 +5,80 @@ open Steel.SelectorEffect
 
 open FStar.Tactics
 
+let lemma_sl_implies_refl (p:viewables) : Lemma
+  (ensures p `sl_implies` p)
+  = admit()
+
+let vemp' : viewable =
+  { fp = emp;
+    a = unit;
+    sel = fun _ -> () }
+
+let vemp : viewables = VUnit vemp'
+
+let emp_unit_variant (#a:Type) (p:a -> viewables) : Lemma
+   (ensures can_be_split_forall (fun x -> p x `star` vemp) p)
+  = admit()
+
+module AE = FStar.Algebra.CommMonoid.Equiv
+module CE = FStar.Tactics.CanonCommMonoidSimple.Equiv
+
+assume val equiv (p1 p2:viewables) : Type0
+
+let equiv_refl (x:viewables) : Lemma (equiv x x) = admit()
+
+let equiv_sym (x y:viewables) : Lemma
+  (requires equiv x y)
+  (ensures equiv y x)
+  = admit()
+
+let equiv_trans (x y z:viewables) : Lemma
+  (requires equiv x y /\ equiv y z)
+  (ensures equiv x z)
+  = admit()
+
+let equiv_sl_implies (p1 p2:viewables) : Lemma
+  (requires p1 `equiv` p2)
+  (ensures p1 `sl_implies` p2)
+  = admit()
+
+inline_for_extraction noextract let req : AE.equiv viewables =
+  AE.EQ equiv
+     equiv_refl
+     equiv_sym
+     equiv_trans
+
+let cm_identity (x:viewables) : Lemma ((vemp `star` x) `equiv` x)
+  = admit()
+
+let star_associative (x y z:viewables) : Lemma (
+  ((x `star` y) `star` z) `equiv` (x `star` (y `star` z)))
+  = admit()
+
+let star_commutative (x y:viewables) : Lemma ((x `star` y) `equiv` (y `star` x))
+  = admit()
+
+let star_congruence (x y z w:viewables) : Lemma
+  (requires (x `equiv` z /\ y `equiv` w))
+  (ensures ((x `star` y) `equiv` (z `star` w)))
+  = admit()
+
+//[@@__reduce__]
+inline_for_extraction noextract let rm : AE.cm viewables req =
+  AE.CM vemp
+     star
+     cm_identity
+     star_associative
+     star_commutative
+     star_congruence
+
+inline_for_extraction noextract let canon_viewables () : Tac unit =
+  CE.canon_monoid (`req) (`rm)
+
+let canon' (_:unit) : Tac unit =
+  or_else (fun _ -> canon_viewables())
+          (fun _ -> fail "Could not prove slprop equivalence")
+
 let rec slterm_nbr_uvars (t:term) : Tac int =
   match inspect t with
   | Tv_Uvar _ _ -> 1
@@ -24,50 +98,143 @@ let rec filter_goals (l:list goal) : Tac (list goal) =
       | App t _ -> if term_eq t (`squash) then hd::filter_goals tl else filter_goals tl
       | _ -> filter_goals tl
 
-let rec solve_next (l:list goal) : Tac bool =
+let rec solve_triv_eqs (l:list goal) : Tac unit =
   match l with
-  | [] -> false
-  | hd::tl -> match term_as_formula' (goal_type hd) with
+  | [] -> ()
+  | hd::tl ->
+    let f = term_as_formula' (goal_type hd) in
+    match f with
     | Comp (Eq _) l r ->
       let lnbr = slterm_nbr_uvars l in
       let rnbr = slterm_nbr_uvars r in
-      if lnbr = 0 || rnbr = 0 then (focus trefl; true) else (later(); solve_next tl)
-    | App _ t -> begin
-      match term_as_formula' t with
-      | Comp (Eq _) l r ->
-      let lnbr = slterm_nbr_uvars l in
-      let rnbr = slterm_nbr_uvars r in
-      if lnbr = 0 || rnbr = 0 then (focus trefl; true) else (later(); solve_next tl)
-      | _ -> false
-      end
-    | _ -> fail "test"; false
+      // Only solve equality if there is only one uvar
+      if lnbr = 0 || rnbr = 0 then trefl () else later();
+      solve_triv_eqs tl
+    | _ -> later(); solve_triv_eqs tl
 
+let solve_can_be_split (args:list argv) : Tac bool =
+  match args with
+  | [(t1, _); (t2, _)] ->
+      let lnbr = slterm_nbr_uvars t1 in
+      let rnbr = slterm_nbr_uvars t2 in
+      if lnbr + rnbr <= 1 then (
+        let open FStar.Algebra.CommMonoid.Equiv in
+        focus (fun _ -> norm [delta_only [`%can_be_split]];
+                     // If we have exactly the same term on both side,
+                     // equiv_sl_implies would solve the goal immediately
+                     or_else (fun _ -> apply_lemma (`lemma_sl_implies_refl))
+                      (fun _ -> apply_lemma (`equiv_sl_implies);
+                       norm [delta_only [
+                              `%__proj__CM__item__unit;
+                              `%__proj__CM__item__mult;
+                              `%Steel.Memory.Tactics.rm;
+                              `%__proj__Mktuple2__item___1; `%__proj__Mktuple2__item___2;
+                              `%fst; `%snd];
+                            primops; iota; zeta];
+                       canon' ()));
+        true
+      ) else false
+
+  | _ -> false // Ill-formed can_be_split, should not happen
+
+let solve_can_be_split_forall (args:list argv) : Tac bool =
+  match args with
+  | [_; (t1, _); (t2, _)] ->
+      let lnbr = slterm_nbr_uvars t1 in
+      let rnbr = slterm_nbr_uvars t2 in
+      if lnbr + rnbr <= 1 then (
+        let open FStar.Algebra.CommMonoid.Equiv in
+        focus (fun _ -> ignore (forall_intro());
+                     norm [delta_only [`%can_be_split_forall]];
+                     or_else (fun _ -> apply_lemma (`lemma_sl_implies_refl))
+                       (fun _ ->
+                       apply_lemma (`equiv_sl_implies);
+                       or_else (fun _ ->  flip()) (fun _ -> ());
+                       norm [delta_only [
+                              `%__proj__CM__item__unit;
+                              `%__proj__CM__item__mult;
+                              `%Steel.Memory.Tactics.rm;
+                              `%__proj__Mktuple2__item___1; `%__proj__Mktuple2__item___2;
+                              `%fst; `%snd];
+                            primops; iota; zeta];
+                       canon' ()));
+        true
+      ) else false
+
+  | _ -> false // Ill-formed can_be_split, should not happen
+
+
+// Returns true if the goal has been solved, false if it should be delayed
+let solve_or_delay (g:goal) : Tac bool =
+  let f = term_as_formula' (goal_type g) in
+  match f with
+  | App _ t ->
+      let hd, args = collect_app t in
+      if term_eq hd (quote delay) then false
+      else if term_eq hd (quote can_be_split) then solve_can_be_split args
+      else if term_eq hd (quote can_be_split_forall) then solve_can_be_split_forall args
+      else false
+  | Comp (Eq _) l r ->
+    let lnbr = slterm_nbr_uvars l in
+    let rnbr = slterm_nbr_uvars r in
+    // Only solve equality if one of the terms is completely determined
+    if lnbr = 0 || rnbr = 0 then (trefl (); true) else false
+  | _ -> fail "unexpected goal"; false
+
+
+// Returns true if it successfully solved a goal
+// If it returns false, it means it didn't find any solvable goal,
+// which should mean only delayed goals are left
+let rec pick_next (l:list goal) : Tac bool =
+  match l with
+  | [] -> false
+  | a::q -> if solve_or_delay a then true else (later (); pick_next q)
+
+
+
+let rec solve_subcomp_post (l:list goal) : Tac unit =
+  match l with
+  | [] -> ()
+  | hd::tl ->
+    let f = term_as_formula' (goal_type hd) in
+    match f with
+    | App _ t ->
+        let hd, args = collect_app t in
+        if term_eq hd (quote annot_sub_post) then (focus (fun _ ->
+          norm [delta_only [`%annot_sub_post]];
+          // Assuming for now that the body will always be Steel
+          // instead of SteelF, as we'll lift pure to Steel by
+          // a polymonadic bind with Steel alloc/read/...
+          // That means the postcondition of return will be ?u_ret * ?u_emp
+          apply_lemma (`emp_unit_variant)
+          ))
+        else (later());
+        solve_subcomp_post tl
+    | _ -> later(); solve_subcomp_post tl
 
 let rec resolve_sel_rec () : Tac unit =
-  if solve_next (goals()) then resolve_sel_rec()
+  match goals () with
+  | [] -> ()
+  | g -> if pick_next g then resolve_sel_rec ()
+        else (norm [delta_only [`%delay]]; resolve_sel_rec ())
 
 [@@ resolve_implicits; framing_implicit_sel]
 let resolve_sel () : Tac unit =
   let gs = filter_goals (goals()) in
   set_goals gs;
-  dump "all goals";
+  solve_triv_eqs (goals());
+  solve_subcomp_post (goals());
   resolve_sel_rec ()
 
 assume val ref : Type0
 assume val ptr (_:ref) : hprop u#1
 assume val sel (r:ref) : projection int (ptr r)
 
-let vemp' : viewable =
-  { fp = emp;
-    a = unit;
-    sel = fun _ -> () }
-
 let vptr' (r:ref) : viewable =
   { fp = ptr r;
     a = int;
     sel = sel r }
 
-let vemp : viewables = VUnit vemp'
 let vptr (r:ref) : viewables = VUnit (vptr' r)
 
 assume val alloc (x:int) : Steel_Sel ref vemp (fun r -> vptr r)
@@ -94,3 +261,12 @@ let test1 (x:int) : Steel_Sel ref vemp vptr (fun _ -> True) (fun _ _ _ -> True) 
   let y = alloc x in
   h_assert (vptr y) (fun _ -> True);
   ret y vptr
+
+let test8 (x:ref) : Steel_Sel int (vptr x) (fun _ -> vptr x) (fun _ -> True) (fun _ _ _ -> True)
+  = let v = read x in
+    let y = alloc v in
+    let v = read y in
+    free y;
+    // Can mix assertions
+    assert (1 == 1);
+    v
